Flapjack/Tests.lean
@@ -1738,4 +1738,13 @@ example :
           (.return (.const 1)) (.return (.const 0))) = some [1] := by
   native_decide
 
+example :
+    (evalPanMemProgFuel 4
+      (fun _ => none)
+      (fun address => if address == 4 then some 7 else none)
+      (.ite (.cmp .equal (.load .one (.const 4)) (.const 7))
+        (.return (.const 1)) (.return (.const 0)))).map
+      (fun result => result.2.2) = some [1] := by
+  native_decide
+
 end Flapjack
